
% this file is called up by thesis.tex
% content in this file will be fed into the main document
    \graphicspath{{Background_Folder/figures/PNG/}{Background_Folder/figures/PDF/}{Background_Folder/figures/}}

%: ———————-- introduction file header ———————--
\chapter{Vortices in U(2) and SU(2) Chern-Simons scalar theories.}



Non-abelian vortices have been studied in \cite{deVega1986, Kumar1986, 1306.5146, NavarroLrida2010}. These have been notably different since the scalars appearing in those models, are in the adjoint representation. This allows for the VEV to remain invariant under the center of the gauge group. If $z\in Z(G)$, where $Z(G)$ is the center of $G$, then by definition $z$ commutes with all elements in the algebra. Thus if an adjoint scalar $\Phi$ has a non-zero VEV, then under a gauge transformation generated by z, we have $\Phi \rightarrow z\Phi z^{\dag} =\Phi z z^{\dag} = \Phi$. In the above cases, the gauge group is $SU(N)$ with center $\mathbb{Z}_N$. In contrast to these studies, we will be interested in fundamental scalars so this argument does not apply directly our subject matter. However, due to the appearance of a non-zero chemical potential, we have found out that non-zero VEVs in the gauge sector come to play a role. Since the gauge fields are in the adjoint representation, this allows for the same type of argument for topological stability to reappear in a theory with fundamental matter. In the context of Yang-Mills theory, this type of vortex has been explored by \cite{hep-ph/0512203}.\\  
Miransky \textit{et al} non-zero chemical potential papers \cite{hep-ph/0512203, Gusynin2004}


\section{U(2) theory}

The action for the $U(2)$ theory can be written down as follows.
\begin{align}
    S^{\text{SU(2)}}_{\text{CS}} &= \frac{k}{4 \pi} \int d^3x \; \epsilon^{\mu \nu \rho} \; \mathrm{Tr} \left[A_{\mu} \partial_{\nu}A_{\rho}+ \frac{2}{3} A_{\mu} A_{\nu}A_{\rho} \right], \\
    S^{\text{U(1)}}_{\text{CS}} &= \frac{k'}{4 \pi} \int d^3x \; \epsilon^{\mu \nu \rho} B_{\mu} \partial_{\nu} B_{\rho},\\
    S_{\text{matter}}&= - \int d^3x \left[ \left(D_{\mu} \Phi \right)^{\dag} \left(D^{\mu} \Phi \right) + V\left(\Phi^{\dag}\Phi \right)\right], \\
    S &= S^{\text{SU(2)}}_{\text{CS}} + S^{\text{U(1)}}_{\text{CS}} + S_{\text{matter}}, \\
    D_{\mu} &= \partial_{\mu} + A_{\mu}+B_{\mu}.
\end{align}
This leads to the classical equations of motion.
\begin{align}
    \frac{k}{2 \pi} F_{\mu \nu} = \epsilon_{\mu \nu \lambda} J^{\lambda}\\
    \frac{k'}{2\pi} f_{\mu \nu} = \epsilon_{\mu \nu \lambda} \frac{1}{2} \mathrm{Tr} \left[\hat{J}^{\lambda} \right],
\end{align}
where
\begin{align}
    F_{\mu \nu}&= \partial_{\mu} A_{\nu} - \partial_{\nu}A_{\mu} + [A_{\mu}, A_{\nu}], \qquad f_{\mu \nu} = \partial_{\mu} B_{\nu} - \partial_{\nu} B_{\mu}, \\
    \hat{J}^{\lambda} &= \sqrt{-g} g^{\lambda \nu} \left( \Phi \left( D_{\nu} \Phi\right)^{\dag} - D_{\nu} \Phi \Phi^{\dag}   -2i \mu_B \delta^0_{\nu} \Phi \Phi^{\dag}  \right), \\
    J^{\lambda} &= \hat{J}^{\lambda} - \frac{1}{2}\mathrm{Tr}\left[\hat{J}^{\lambda} \right]\mathbb{I} \qquad \implies \qquad \mathrm{Tr}\left[J^{\lambda}\right]=0.
\end{align}
More explicitly the equations become
\begin{align}
    \frac{k}{2\pi} \left(\partial_r A_{\theta} - \partial_{\theta} A_r + [A_r, A_{\theta}]\right) &= r \big\lbrace (A_0 +B_0+ i \mu_B ) , \Phi \Phi^{\dag} \big\rbrace - \frac{1}{2} \mathrm{Tr} \left[ \hat{J}^0 \right] \\
    \frac{k}{2\pi} \left(\partial_0 A_r - \partial_r A_0 + [A_0, A_r]\right) &= -\frac{1}{r} \left(\partial_{\theta} \Phi \Phi^{\dag} -\Phi \partial_{\theta}\Phi^{\dag} + \big\lbrace (A_{\theta} +B_{\theta}), \Phi \Phi^{\dag} \big\rbrace \right) - \frac{1}{2} \mathrm{Tr} \left[ \hat{J}^{\theta} \right]\\
    \frac{k}{2 \pi} \left(\partial_{\theta} A_0 - \partial_{0} A_{\theta} + [A_{\theta}, A_0]\right) &=-r \left(\partial_{r} \Phi \Phi^{\dag} \Phi \partial_r \Phi^{\dag} + \big\lbrace (A_r +B_r), \Phi \Phi^{\dag} \big\rbrace \right) - \frac{1}{2} \mathrm{Tr} \left[ \hat{J}^r \right]. \\
    \frac{k'}{2 \pi} \left( \partial_r B_{\theta}- \partial_{\theta} B_r\right) &= \frac{1}{2} \mathrm{Tr} [\hat{J}^0]\\
    \frac{k'}{2 \pi} \left( \partial_0 B_{r}- \partial_{r} B_0\right) &= \frac{1}{2} \mathrm{Tr} [\hat{J}^{\theta}]\\
    \frac{k'}{2 \pi} \left( \partial_{\theta} B_{0}- \partial_{0} B_{\theta}\right) &= \frac{1}{2} \mathrm{Tr} [\hat{J}^r]\\
\end{align}
Inserting the ansatz
\begin{align}
    A_{\mu} &= i \left(a_{\mu}^3 \sigma_3 + a_{\mu}^+ \sigma_{+} +a_{\mu}^{-} \sigma_{-} \right), \\
    B_{\mu} &= i \left( a_{\mu} \mathbb{I} \right), \\
    \Phi &=  e^{i n \theta} \begin{pmatrix}
        0\\
        \varphi(r)\\
    \end{pmatrix}, \qquad n\in \mathbb{Z}, \qquad \varphi(r) \xrightarrow{r \rightarrow \infty} v,
\end{align}
    where
    \begin{align}
        \sigma_3 = \begin{bmatrix}
            1 & 0 \\
            0 & -1 \\
        \end{bmatrix}, \qquad \mathbb{I}= \begin{bmatrix}
            1 & 0\\
            0 & 1\\
        \end{bmatrix} \\
        \sigma_+ =\begin{bmatrix}
            0 & 1\\
            0 & 0\\
        \end{bmatrix}, \qquad \sigma_- = \begin{bmatrix}
            0 &0\\
            1 &0\\
        \end{bmatrix}
    \end{align}
    \begin{align}
        \Phi \Phi^{\dag} = \varphi(r)^2 \begin{pmatrix} 
            0 & 0\\
            0 & 1\\
        \end{pmatrix} = \varphi(r)^2 \sigma_- \sigma_+.
    \end{align}

    And using the following relations in order to simplify the equations of motion.
    \begin{align}
        [\sigma_+, \sigma_-] = \sigma_3, \qquad [\sigma_3, \sigma_+] = 2 \sigma_+, \qquad [\sigma_3, \sigma_-] = -2 \sigma_-.
    \end{align}

    The gauge equations of motion become

    \begin{align}
        \frac{k}{2 \pi} \left(\partial_{r} a_{\theta}^3 - \partial_{\theta} a_r^{(3)} + i \left(a_r^+ a_{\theta}^- - a_r^- a_{\theta}^{+} \right) \right) &= -r \left( a_0 + \mu - a^{(3)}_0 \right)\varphi^2 \\
        \frac{k}{2 \pi} \left(\partial_r a_{\theta}^{+} - \partial_{\theta} a_r^{+} +2i \left(a_r^{(3)} a_{\theta}^{+} - a_r^{+} a_{\theta}^{(3)} \right) \right) &=r a_0^{+} \varphi^2  \\
        \frac{k'}{2 \pi} \left(\partial_r a_{\theta} - \partial_{\theta} a_r \right) &=r \left(a_0 +\mu - a^{(3)}_0 \right) \varphi^2 + r J_0  \\
        \frac{k}{2 \pi}\left(\partial_{0}a_r^{(3)} - \partial_r a_0^{(3)} + i \left(a_0^+ a_r^- - a_0^- a_r^+  \right)  \right) &= \frac{1}{r} \left(a_{\theta}+n - a_{\theta}^{(3)} \right) \varphi^2  \\
        \frac{k}{2 \pi} \left( \partial_0 a_r^+ - \partial_r a_0^+ + 2i \left( a_0^{(3)} a_r^+ -a_0^+ a_r^{(3)} \right) \right) &= -\frac{1}{r} a_{\theta}^+ \varphi^2  \\
        \frac{k'}{2 \pi} \left( \partial_0 a_r - \partial_r a_0 \right) &= -\frac{1}{r} \left(a_{\theta} +n - a_{\theta}^{(3)} \right) \varphi^2 \\
        \frac{k}{2 \pi} \left(\partial_{\theta} a_0^{(3)} - \partial_0 a_{\theta}^{(3)} + i \left(a_{\theta}^+ a_0^- - a_{\theta}^- a_0^{+} \right) \right) &= r \left(a_r - a_r^{(3)}  \right) \varphi^2 \\
        \frac{k}{2 \pi} \left(\partial_{\theta} a_0^+ - \partial_0 a_{\theta}^+ + 2i \left(a_{\theta}^{(3)} a_0^+ - a_{\theta}^+ a_0^{(3)} \right) \right) &=-r a_r^+ \varphi^2\\
        \frac{k'}{2 \pi} \left(\partial_{\theta}a_0 -\partial_{0} a_{\theta} \right) &= r \left(a_r^{(3)}- a_r \right) \varphi^2,
    \end{align}
    where $J_0$ is determined by requiring that the system is neutral when evaluated at the VEV. This implies that
    \begin{align}
        J_0 = -\frac{\pi v^2}{k} \left(\frac{\mu k}{\pi}- v^2 \right) .
    \end{align}
    For static solutions, we may take
    \begin{align}
        a_{\mu}^{(3)} = f_{\mu}(r), \qquad a_{\mu}^+ = g_{\mu}(r)e^{-i \theta},\qquad a_{\mu}^- = g_{\mu}^*(r) e^{i \theta}, \qquad a_{\mu} = a_{\mu}(r).
    \end{align}
    With this ansatz, we have
    \begin{align}
        \frac{k}{2\pi} \left(f_{\theta}'(r) +i \left(g_r g_{\theta}^* - g_r^* g_{\theta} \right) \right) &= -r \left(a_0 +\mu - f_0 \right)\phi^2 \\
        \frac{k}{2 \pi} \left(g_{\theta}'(r) - i g_r +2i \left(f_r g_{\theta} -g_r f_{\theta} \right) \right) &=r g_0 \phi^2 \\
        \frac{k'}{2\pi} a_{\theta}' &= r \left(a_0 + \mu -f_0\right)\phi^2 -r J_0\\
        \frac{k}{2\pi} \left(f_0' + i \left(g_0 g_r^* - g_0^* g_r\right)\right)&= \frac{1}{r} \left(a_{\theta} + n - f_{\theta}\right)\phi^2\\
        \frac{k}{2\pi} \left(g_0' - 2i \left(f_0 g_r - g_0 f_r \right)\right) &= \frac{1}{r} g_{\theta} \phi^2\\
        \frac{k'}{2\pi} a_0' &=\frac{1}{r} \left(a_{\theta} +n - f_{\theta}\right) \phi^2 \\
        \frac{i k}{2\pi} \left(g_{\theta}g_0^* - g_{\theta}^* g_0\right) &= r \left(a_r -f_r\right) \phi^2 \\
        \frac{i k}{2\pi} \left(  g_0 - 2 \left(f_{\theta} g_0 - g_{\theta} f_0 \right)\right) &= r g_r \phi^2\\
        r \left(f_r -a_r\right) \phi^2 &= 0.
    \end{align}
    From these equations we can see that we can further restrict the ansatz \textcolor{red}{(include this in the appendix)} so that
    \begin{align}
        f_r &=a_r = 0 \\
        g_0(r) = \tilde{g}_0(r) e^{i \alpha}, \qquad g_{\theta}(r) &= \tilde{g}_{\theta}(r) e^{i \alpha}, \qquad g_r(r) =  \tilde{g}_r(r) e^{i \left(\alpha + \frac{\pi}{2} \right)},
    \end{align}
    where all of $\tilde{g}_{\mu} \in \mathbb{R}$. Note the $\frac{\pi}{2}$ shift of the phase of the $g_r$ component relative to the rest of the functions. This is analogous to how the vacuum components of $A_{\theta}$ and $A_r$ relate to one another. The phase factor $e^{i \alpha}$ has to do with the remaining gauge freedom in the system.
    The system of equations then simplifies to
    \begin{align}
        \frac{k}{2 \pi } \left(f_{\theta}' - 2\tilde{g}_r \tilde{g}_{\theta}\right) &= -r \left(a_0 + \mu - f_0\right) \phi^2\\
        \frac{k}{2 \pi} \left(\tilde{g}_{\theta}' + \tilde{g}_r - 2 \tilde{g}_r f_{\theta} \right) & = r\tilde{g}_0 \phi^2 \\
        \frac{k'}{2 \pi} a_{\theta}' &= r \left(a_0 +\mu - f_0 \right)\phi^2 - rJ_0 \\
        \frac{k}{2\pi} \left(f_0'+2 \tilde{g}_0\tilde{g}_r\right) &= \frac{1}{r} \left(a_{\theta}+n - f_{\theta}\right)\phi^2 \\
        \frac{k}{2\pi}\left(\tilde{g}_0' + 2 f_0 \tilde{g}_r \right) &=\frac{1}{r} \tilde{g}_{\theta}\phi^2 \\
        \frac{k'}{2\pi} a_0'&= \frac{1}{r} \left(a_{\theta}+n - f_{\theta}\right) \phi^2 \\
        \frac{k}{2\pi} \left(\tilde{g}_0 - 2\left(f_{\theta} \tilde{g}_0 - \tilde{g}_{\theta} f_0\right)\right) &= r \tilde{g}_r \phi^2.
    \end{align}
\section{SU(2) theory}

The $SU(2)$ equations of motion are determined by requiring that the trace of the $U(2)$ equations of motion vanishes. This leads to the simplified system
    \begin{align}
        \frac{k}{2 \pi} \left(\partial_{r} a_{\theta}^3 - \partial_{\theta} a_r^{(3)} + i \left(a_r^+ a_{\theta}^- - a_r^- a_{\theta}^{+} \right) \right) &= -r \left(\mu - a^{(3)} \right)\phi^2 \\
        \frac{k}{2 \pi} \left(\partial_r a_{\theta}^{+} - \partial_{\theta} a_r^{+} +2i \left(a_r^{(3)} a_{\theta}^{+} - a_r^{+} a_{\theta}^{(3)} \right) \right) &=r a_0^{+} \phi^2  \\
        \frac{k}{2 \pi}\left(\partial_{0}a_r^{(3)} - \partial_r a_0^{(3)} + i \left(a_0^+ a_r^- - a_0^- a_r^+  \right)  \right) &= \frac{1}{r} \left(n - a_{\theta}^{(3)} \right) \phi^2  \\
        \frac{k}{2 \pi} \left( \partial_0 a_r^+ - \partial_r a_0^+ + 2i \left( a_0^{(3)} a_r^+ -a_0^+ a_r^{(3)} \right) \right) &= -\frac{1}{r} a_{\theta}^+ \phi^2  \\
        \frac{k}{2 \pi} \left(\partial_{\theta} a_0^{(3)} - \partial_0 a_{\theta}^{(3)} + i \left(a_{\theta}^+ a_0^- - a_{\theta}^- a_0^{+} \right) \right) &= -r  a_r^{(3)} \phi^2 \\
        \frac{k}{2 \pi} \left(\partial_{\theta} a_0^+ - \partial_0 a_{\theta}^+ + 2i \left(a_{\theta}^{(3)} a_0^+ - a_{\theta}^+ a_0^{(3)} \right) \right) &=-r a_r^+ \phi^2\\
    \end{align}




